lib/SubMonadLib.thy
@@ -1,4 +1,5 @@
 (*
+ * Copyright 2025, Proofcraft Pty Ltd
  * Copyright 2020, Data61, CSIRO (ABN 41 687 119 230)
  *
  * SPDX-License-Identifier: BSD-2-Clause
@@ -7,57 +8,56 @@
 theory SubMonadLib
 imports
   Monads.Nondet_Empty_Fail
-  Corres_UL
+  ExtraCorres
 begin
 
 locale submonad_args =
-  fixes fetch :: "'a \<Rightarrow> 'b"
-  fixes replace :: "'b \<Rightarrow> 'a \<Rightarrow> 'a"
-  fixes guard :: "'a \<Rightarrow> bool"
+  fixes fetch :: "('c, 's) monad_state \<Rightarrow> 'b"
+  fixes replace :: "'b \<Rightarrow> ('c, 's) monad_state \<Rightarrow> ('c, 's) monad_state"
+  fixes guard :: "('c, 's) mpred"
 
   assumes args:
-   "\<forall>x s. guard s \<longrightarrow> fetch (replace x s) = x"
-   "\<forall>x y s. replace x (replace y s) = replace x s"
+   "\<forall>x s. guard s \<longrightarrow> fetch (const_env (replace x) s) = x"
+   "\<forall>x y s. replace x (const_env (replace y) s) = replace x s"
    "\<forall>s. replace (fetch s) s = s"
 
   assumes replace_preserves_guard:
-   "\<And>s x. guard (replace x s) = guard s"
+   "\<And>s x. guard (const_env (replace x) s) = guard s"
 
-definition
-  submonad_fn :: "('a \<Rightarrow> 'b) \<Rightarrow> ('b \<Rightarrow> 'a \<Rightarrow> 'a) \<Rightarrow> ('a \<Rightarrow> bool) \<Rightarrow>
-                  ('b, 'c) nondet_monad \<Rightarrow> ('a, 'c) nondet_monad"
-where
- "submonad_fn fetch replace guard m \<equiv> do
-    stateAssert guard [];
-    substate \<leftarrow> gets fetch;
-    (rv, substate') \<leftarrow> select_f (m substate);
-    modify (replace substate');
-    return rv
-  od"
+definition submonad_fn ::
+  "(('c, 's) monad_state \<Rightarrow> 't) \<Rightarrow>
+   ('t \<Rightarrow> ('c, 's) monad_state \<Rightarrow> ('c, 's) monad_state) \<Rightarrow>
+   ('c, 's) mpred \<Rightarrow>
+   (unit, 't, 'r) nondet_monad \<Rightarrow>
+   ('c, 's, 'r) nondet_monad"
+  where
+  "submonad_fn fetch replace guard m \<equiv> do
+     stateAssert guard [];
+     substate \<leftarrow> gets fetch;
+     (rv, substate') \<leftarrow> select_f (m (monad_state () substate));
+     modify (replace substate');
+     return rv
+   od"
 
 locale submonad = submonad_args +
-  fixes fn :: "('b, 'c) nondet_monad \<Rightarrow> ('a, 'c) nondet_monad"
+  fixes fn :: "(unit, 't, 'r) nondet_monad \<Rightarrow> ('c, 's, 'r) nondet_monad"
 
   assumes fn_is_sm: "fn = submonad_fn fetch replace guard"
 
 lemma (in submonad_args) argsD1:
-  "\<And>x s. guard s \<Longrightarrow> fetch (replace x s) = x"
+  "\<And>x s. guard s \<Longrightarrow> fetch (const_env (replace x) s) = x"
   by (simp add: args)
 
 lemma (in submonad) guarded_sm:
   "\<And>s. guard s \<Longrightarrow>
    fn m s = (do
      substate \<leftarrow> gets fetch;
-     (rv, substate') \<leftarrow> select_f (m substate);
+     (rv, substate') \<leftarrow> select_f (m (monad_state () substate));
      modify (replace substate');
      return rv
    od) s"
   unfolding fn_is_sm submonad_fn_def
   by (simp add: stateAssert_def get_def assert_def bind_def return_def)
-
-lemma modify_modify:
-  "modify fn1 >>= (\<lambda>x. modify fn2) = modify (fn2 \<circ> fn1)"
-  by (simp add: bind_def modify_def get_def put_def)
 
 lemma select_f_walk:
   assumes m1: "empty_fail m1"
@@ -91,11 +91,10 @@ lemma stateAssert_stateAssert:
   by (simp add: ext stateAssert_def bind_def get_def assert_def fail_def return_def)
 
 lemma modify_stateAssert:
-  "\<lbrakk> \<And>s x. g (r x s) = g s \<rbrakk> \<Longrightarrow>
-   (modify (r x) >>= (\<lambda>u. stateAssert g []))
-            = (stateAssert g [] >>= (\<lambda>u. modify (r x)))"
+  "\<lbrakk> \<And>s x. g (const_env (r x) s) = g s \<rbrakk> \<Longrightarrow>
+   (modify (r x) >>= (\<lambda>u. stateAssert g [])) = (stateAssert g [] >>= (\<lambda>u. modify (r x)))"
   by (simp add: ext stateAssert_def bind_def get_def assert_def fail_def
-                return_def modify_def put_def)
+                return_def modify_def put_def const_env_def)
 
 lemma gets_stateAssert:
   "(gets f >>= (\<lambda>x. stateAssert g' [] >>= (\<lambda>u. m x)))
@@ -117,38 +116,12 @@ lemma select_f_stateAssert:
   apply fastforce
   done
 
-lemma bind_select_f_bind':
-  shows "(select_f (m s) >>= (\<lambda>x. select_f (split n x))) = (select_f ((m >>= n) s))"
-  apply (rule ext)
-  apply (force simp: select_f_def bind_def split_def)
-  done
-
-lemma bind_select_f_bind:
-  "(select_f (m1 s) >>= (\<lambda>x. select_f (m2 (fst x) (snd x)))) = (select_f ((m1 >>= m2) s))"
-  by (insert bind_select_f_bind' [where m=m1 and n=m2 and s=s],
-      simp add: split_def)
-
-lemma select_from_gets: "select_f (gets f s) = return (f s, s)"
-  apply (rule ext)
-  apply (simp add: select_f_def return_def simpler_gets_def)
-  done
-
-lemma select_from_gets':
-  "(select_f \<circ> gets f) = (\<lambda>s. return (f s, s))"
-  apply (rule ext)
-  apply (simp add: o_def select_from_gets)
-  done
-
-lemma bind_subst_lift:
-  "(f >>= g) = h \<Longrightarrow> (do x \<leftarrow> f; y \<leftarrow> g x; j y od) = (h >>= j)"
-  by (simp add: bind_assoc[symmetric])
-
 lemma modify_gets:
-  "\<lbrakk> \<And>x s. g (r x s) = g s; \<And>x s. g s \<longrightarrow> f (r x s) = x \<rbrakk>
+  "\<lbrakk> \<And>x s. g (const_env (r x) s) = g s; \<And>x s. g s \<longrightarrow> f (const_env (r x) s) = x \<rbrakk>
    \<Longrightarrow> (modify (r x) >>= (\<lambda>u. stateAssert g [] >>= (\<lambda>u'. gets f)))
             = (stateAssert g [] >>= (\<lambda>u'. modify (r x) >>= (\<lambda>u. return x)))"
   by (simp add: ext stateAssert_def assert_def modify_def bind_def get_def
-                put_def gets_def return_def fail_def)
+                put_def gets_def return_def fail_def const_env_def)
 
 lemma (in submonad_args) gets_modify:
   "\<And>s. guard s \<Longrightarrow>
@@ -174,48 +147,49 @@ lemma submonad_bind:
   done
 
 lemma (in submonad) guard_preserved:
-  "\<And>s s'. \<lbrakk> (rv, s') \<in> fst (fn m s) \<rbrakk> \<Longrightarrow> guard s'"
+  "\<And>s s'. \<lbrakk> (rv, s') \<in> fst (fn m s) \<rbrakk> \<Longrightarrow> guard (with_env_of s s')"
   unfolding fn_is_sm submonad_fn_def
-  by (clarsimp simp: stateAssert_def gets_def get_def bind_def modify_def put_def
-                     return_def select_f_def replace_preserves_guard in_monad)
+  by (clarsimp simp: stateAssert_def gets_def get_def bind_def modify_def put_def return_def
+                     select_f_def replace_preserves_guard[unfolded const_env_def] in_monad)
 
 lemma fst_stateAssertD:
-  "\<And>s s' v. (v, s') \<in> fst (stateAssert g [] s) \<Longrightarrow> s' = s \<and> g s"
+  "\<And>s s' v. (v, s') \<in> fst (stateAssert g [] s) \<Longrightarrow> s' = mstate s \<and> g s"
   by (clarsimp simp: stateAssert_def in_monad)
 
 lemma(in submonad) guarded_gets:
-  "\<And>s. guard s \<Longrightarrow> fn (gets f) s = gets (f \<circ> fetch) s"
+  "\<And>s. guard s \<Longrightarrow> fn (gets f) s = gets (f \<circ> monad_state () \<circ> fetch) s"
   apply (simp add: guarded_sm select_from_gets gets_modify)
   apply (simp add: gets_def)
   done
 
 lemma (in submonad) guarded_return:
   "\<And>s. guard s \<Longrightarrow> fn (return x) s = return x s"
-  using args guarded_gets
+  using args guarded_gets guarded_sm
   by (fastforce simp: gets_def bind_def get_def)
 
 lemma (in submonad_args) submonad_fn_gets:
   "submonad_fn fetch replace guard (gets f) =
-   (stateAssert guard [] >>= (\<lambda>u. gets (f \<circ> fetch)))"
+   (stateAssert guard [] >>= (\<lambda>u. gets (f \<circ> monad_state () \<circ> fetch)))"
   apply (simp add: ext select_from_gets submonad_fn_def)
   apply (rule bind_cong [OF refl])
   apply (clarsimp simp: gets_modify dest!: fst_stateAssertD)
   apply (simp add: gets_def)
   done
 
-lemma(in submonad) gets:
-  "fn (gets f) = (stateAssert guard [] >>= (\<lambda>u. gets (f \<circ> fetch)))"
+lemma (in submonad) gets:
+  "fn (gets f) = (stateAssert guard [] >>= (\<lambda>_. gets (f \<circ> monad_state () \<circ> fetch)))"
   unfolding fn_is_sm submonad_fn_gets
   by (rule refl)
 
 lemma (in submonad) return:
-  "fn (return x) = (stateAssert guard [] >>= (\<lambda>u. return x))"
+  "fn (return x) = (stateAssert guard [] >>= (\<lambda>_. return x))"
   using args gets
-  by (fastforce simp: gets_def bind_def get_def)
+  by (fastforce simp: gets_def bind_def get_def return_def)
 
 lemma (in submonad) mapM_guard_preserved:
-  "\<And>s s'. \<lbrakk> guard s; \<exists>rv. (rv, s') \<in> fst (mapM (fn \<circ> m) xs s)\<rbrakk> \<Longrightarrow> guard s'"
-proof (induct xs)
+  "\<lbrakk> guard (with_env_of t s); \<exists>rv. (rv, s') \<in> fst (mapM (fn \<circ> m) xs (with_env_of t s))\<rbrakk> \<Longrightarrow>
+   guard (with_env_of t s')"
+proof (induct xs arbitrary: s)
   case Nil
   thus ?case
     by (simp add: mapM_def sequence_def return_def)
@@ -229,8 +203,9 @@ proof (induct xs)
 qed
 
 lemma (in submonad) mapM_x_guard_preserved:
-  "\<And>s s'. \<lbrakk> guard s; \<exists>rv. (rv, s') \<in> fst (mapM_x (fn \<circ> m) xs s)\<rbrakk> \<Longrightarrow> guard s'"
-proof (induct xs)
+  "\<lbrakk> guard (with_env_of t s); \<exists>rv. (rv, s') \<in> fst (mapM_x (fn \<circ> m) xs (with_env_of t s))\<rbrakk> \<Longrightarrow>
+   guard (with_env_of t s')"
+proof (induct xs arbitrary: s)
   case Nil
   thus ?case
     by (simp add: mapM_x_def sequence_x_def return_def)
@@ -252,10 +227,10 @@ lemma (in submonad) fn_stateAssert:
   "fn m >>= (\<lambda>x. stateAssert guard [] >>= (\<lambda>u. n x)) = (fn m >>= n)"
   apply (simp add: fn_is_sm submonad_fn_def bind_assoc split_def)
   apply (rule ext)
-  apply (rule bind_apply_cong [OF refl])+
+  apply (rule bind_apply_cong[OF refl])+
   apply (clarsimp simp: stateAssert_def bind_assoc in_monad select_f_def)
-  apply (drule iffD2 [OF replace_preserves_guard])
-  apply (fastforce simp: bind_def assert_def get_def return_def)
+  apply (drule iffD2[OF replace_preserves_guard])
+  apply (fastforce simp: bind_def assert_def get_def return_def const_env_def)
   done
 
 lemma submonad_mapM:
@@ -276,9 +251,10 @@ proof (induct l)
     apply (simp add: bind_assoc submonad_bind submonad.return empty_fail_cond)
     apply (subst submonad.fn_stateAssert [OF sm'])
     apply (intro ext bind_apply_cong [OF refl])
-    apply (subgoal_tac "g sta")
+    apply (rename_tac s rv st rv' st')
+    apply (subgoal_tac "g (with_env_of s st')")
      apply (clarsimp simp: stateAssert_def bind_def get_def assert_def return_def)
-    apply (frule(1) submonad.guard_preserved)
+    apply (frule (1) submonad.guard_preserved)
     apply (erule(1) submonad.mapM_guard_preserved, fastforce simp: o_def)
     done
 qed
@@ -301,14 +277,15 @@ proof (induct l)
     apply (simp add: bind_assoc submonad_bind submonad.return)
     apply (subst submonad.fn_stateAssert [OF sm'])
     apply (intro ext bind_apply_cong [OF refl])
-    apply (subgoal_tac "g st")
+    apply (rename_tac s rv st)
+    apply (subgoal_tac "g (with_env_of s st)")
      apply (clarsimp simp: stateAssert_def bind_def get_def assert_def return_def)
     apply (frule(1) submonad.guard_preserved, simp)
     done
 qed
 
 lemma corres_select:
-  "(\<forall>s' \<in> S'. \<exists>s \<in> S. rvr s s') \<Longrightarrow> corres_underlying sr nf nf' rvr \<top> \<top> (select S) (select S')"
+  "\<forall>s' \<in> S'. \<exists>s \<in> S. rvr s s' \<Longrightarrow> corres_underlying sr nf nf' rvr \<top> \<top> (select S) (select S')"
   by (clarsimp simp: select_def corres_underlying_def)
 
 lemma corres_select_f:
@@ -317,15 +294,9 @@ lemma corres_select_f:
   by (clarsimp simp: select_f_def corres_underlying_def)
 
 lemma corres_modify':
-  "\<lbrakk> (\<forall>s s'. (s, s') \<in> sr \<longrightarrow> (f s, f' s') \<in> sr); r () () \<rbrakk>
+  "\<lbrakk> \<forall>s s'. (s, s') \<in> sr \<longrightarrow> (const_env f s, const_env f' s') \<in> sr; r () () \<rbrakk>
       \<Longrightarrow> corres_underlying sr nf nf' r \<top> \<top> (modify f) (modify f')"
-  by (clarsimp simp: modify_def corres_underlying_def bind_def get_def put_def)
-
-(* FIXME: this should only be used for the lemma below *)
-lemma corres_select_f_stronger:
-  "\<lbrakk> \<forall>s' \<in> fst S'. \<exists>s \<in> fst S. rvr s s'; nf' \<Longrightarrow> \<not> snd S' \<rbrakk>
-      \<Longrightarrow> corres_underlying sr nf nf' rvr \<top> \<top> (select_f S) (select_f S')"
-  by (clarsimp simp: select_f_def corres_underlying_def)
+  by (clarsimp simp: modify_def corres_underlying_def bind_def get_def put_def const_env_def)
 
 lemma stateAssert_sp:
   "\<lbrace>P\<rbrace> stateAssert Q l \<lbrace>\<lambda>_. P and Q\<rbrace>"
@@ -333,32 +304,34 @@ lemma stateAssert_sp:
 
 lemma corres_submonad:
   "\<lbrakk> submonad f r g fn; submonad f' r' g' fn';
-     \<forall>s s'. (s, s') \<in> sr \<and> g s \<and> g' s' \<longrightarrow> (f s, f' s') \<in> ssr;
-     \<forall>s s' ss ss'. ((s, s') \<in> sr \<and> (ss, ss') \<in> ssr) \<longrightarrow> (r ss s, r' ss' s') \<in> sr;
+     \<forall>s s'. (s, s') \<in> sr \<and> g s \<and> g' s' \<longrightarrow> (monad_state () (f s), monad_state () (f' s')) \<in> ssr;
+     \<forall>s s' ss ss'. (s, s') \<in> sr \<longrightarrow> (ss, ss') \<in> ssr \<longrightarrow> (const_env (r (mstate ss)) s, const_env (r' (mstate ss')) s') \<in> sr;
      corres_underlying ssr False nf' rvr \<top> \<top> x x'\<rbrakk>
    \<Longrightarrow> corres_underlying sr False nf' rvr g g' (fn x) (fn' x')"
   apply (subst submonad.fn_is_sm, assumption)+
   apply (clarsimp simp: submonad_fn_def)
-  apply (rule corres_underlying_split [OF _ _ stateAssert_sp stateAssert_sp])
+  apply (rule corres_underlying_split[OF _ _ stateAssert_sp stateAssert_sp, where r'=dc])
    apply (fastforce simp: corres_underlying_def stateAssert_def get_def
-                         assert_def return_def bind_def)
-  apply (rule corres_underlying_split [where r'="\<lambda>x y. (x, y) \<in> ssr",
-                             OF _ _ hoare_TrueI hoare_TrueI])
+                          assert_def return_def bind_def)
+  apply (rule corres_underlying_split[where r'="\<lambda>x y. (monad_state () x,  monad_state () y) \<in> ssr",
+                                      OF _ _ hoare_TrueI hoare_TrueI])
    apply clarsimp
-  apply (rule corres_underlying_split [where r'="\<lambda>(x, x') (y, y'). rvr x y \<and> (x', y') \<in> ssr",
-                             OF _ _ hoare_TrueI hoare_TrueI])
-   defer
-   apply clarsimp
-   apply (rule corres_underlying_split [where r'=dc, OF _ _ hoare_TrueI hoare_TrueI])
-    apply (simp add: corres_modify')
-   apply clarsimp
-  apply (rule corres_select_f_stronger)
+  apply (rule corres_underlying_split[where
+                r'="\<lambda>(x, x') (y, y'). rvr x y \<and> (monad_state () x', monad_state () y') \<in> ssr",
+                OF _ _ hoare_TrueI hoare_TrueI])
+   apply (rule corres_select_f)
+    apply (clarsimp simp: corres_underlying_def)
+    apply (drule (1) bspec, clarsimp)
+    apply (drule (1) bspec, simp)
+    apply blast
    apply (clarsimp simp: corres_underlying_def)
    apply (drule (1) bspec, clarsimp)
-   apply (drule (1) bspec, simp)
-   apply blast
-  apply (clarsimp simp: corres_underlying_def)
-  apply (drule (1) bspec, clarsimp)
+  apply clarsimp
+  apply (rule corres_underlying_split[where r'=dc, OF _ _ hoare_TrueI hoare_TrueI])
+   apply (rule corres_modify')
+    apply fastforce
+   apply simp
+  apply clarsimp
   done
 
 lemma stateAssert_top [simp]:
@@ -372,18 +345,15 @@ lemma stateAssert_A_top [simp]:
 text \<open>Use of the submonad concept to demonstrate commutativity.\<close>
 
 lemma gets_modify_comm:
-  "\<And> s. \<lbrakk> g (f s) = g s \<rbrakk> \<Longrightarrow>
+  "\<And> s. \<lbrakk> g (const_env f s) = g s \<rbrakk> \<Longrightarrow>
    (do x \<leftarrow> modify f; y \<leftarrow> gets g; m x y od) s =
    (do y \<leftarrow> gets g; x \<leftarrow> modify f; m x y od) s"
-  by (simp add: modify_def gets_def get_def bind_def put_def return_def)
+  by (simp add: modify_def gets_def get_def bind_def put_def return_def const_env_def)
 
 lemma bind_subst_lhs_inv:
   "\<And>s. \<lbrakk> \<And>x s'. P s' \<Longrightarrow> (f x >>= g x) s' = h x s'; \<lbrace>P\<rbrace> a \<lbrace>\<lambda>_. P\<rbrace>; P s \<rbrakk> \<Longrightarrow>
    (do x \<leftarrow> a; y \<leftarrow> f x; g x y od) s = (a >>= h) s"
-  apply (rule bind_apply_cong [OF refl])
-  apply (drule(2) use_valid)
-  apply simp
-  done
+  by (fact monad_eq_split)
 
 lemma gets_comm:
   "do x \<leftarrow> gets f; y \<leftarrow> gets g; m x y od = do y \<leftarrow> gets g; x \<leftarrow> gets f; m x y od"
@@ -392,25 +362,16 @@ lemma gets_comm:
 lemma submonad_comm:
   assumes x1: "submonad_args f r g" and x2: "submonad_args f' r' g'"
   assumes y: "m = submonad_fn f r g im" "m' = submonad_fn f' r' g' im'"
-  assumes z: "\<And>s x x'. r x (r' x' s) = r' x' (r x s)"
-  assumes gp: "\<And>s x. g (r' x s) = g s" and gp': "\<And>s x. g' (r x s) = g' s"
+  assumes z: "\<And>s x x'. r x (const_env (r' x') s) = r' x' (const_env (r x) s)"
+  assumes gp: "\<And>s x. g (const_env (r' x) s) = g s" and gp': "\<And>s x. g' (const_env (r x) s) = g' s"
   assumes efim: "empty_fail im" and efim': "empty_fail im'"
   shows      "(do x \<leftarrow> m; y \<leftarrow> m'; n x y od) = (do y \<leftarrow> m'; x \<leftarrow> m; n x y od)"
 proof -
-  have P: "\<And>x s. g s \<Longrightarrow> f (r' x s) = f s"
-    apply (subgoal_tac "f (r' x (r (f s) s)) = f s")
-     apply (simp add: submonad_args.args[OF x1])
-    apply (simp add: z[symmetric])
-    apply (subst(asm) gp [symmetric])
-    apply (fastforce dest: submonad_args.argsD1[OF x1])
-    done
-  have Q: "\<And>x s. g' s \<Longrightarrow> f' (r x s) = f' s"
-    apply (subgoal_tac "f' (r x (r' (f' s) s)) = f' s")
-     apply (simp add: submonad_args.args[OF x2])
-    apply (simp add: z)
-    apply (subst(asm) gp' [symmetric])
-    apply (fastforce dest: submonad_args.argsD1[OF x2])
-    done
+  have P: "\<And>x s. g s \<Longrightarrow> f (const_env (r' x) s) = f s"
+    by (smt (verit, ccfv_threshold) gp submonad_args_def x1 x2 z)
+  have Q: "\<And>x s. g' s \<Longrightarrow> f' (const_env (r x) s) = f' s"
+    by (smt (verit, ccfv_threshold) const_env_monad_state gp' submonad_args.args(1)
+                                    submonad_args.args(3) surjective x2 z)
   note empty_failD [OF efim, simp]
   note empty_failD [OF efim', simp]
   note empty_fail_select_f[simp]
@@ -422,7 +383,6 @@ proof -
     apply (subst gets_stateAssert bind_subst_lift [OF stateAssert_stateAssert])+
     apply (rule bind_cong)
      apply (simp add: pred_conj_def conj_comms)
-    apply (simp add: bind_assoc select_f_walk[symmetric])
     apply (clarsimp dest!: fst_stateAssertD)
     apply (subst bind_assoc[symmetric],
            subst bind_subst_lhs_inv [OF gets_modify_comm],
@@ -436,15 +396,15 @@ proof -
            rule bind_apply_cong [OF refl])
     apply (subst select_f_walk, simp, simp, rule bind_apply_cong [OF refl])
     apply (clarsimp simp: simpler_gets_def select_f_def)
-    apply (simp add: bind_def get_def put_def modify_def z)
+    apply (simp add: bind_def get_def put_def modify_def z[unfolded const_env_def])
     done
 qed
 
 lemma submonad_comm2:
   assumes x1: "submonad_args f r g" and x2: "m = submonad_fn f r g im"
   assumes y: "submonad f' r' g' m'"
-  assumes z: "\<And>s x x'. r x (r' x' s) = r' x' (r x s)"
-  assumes gp: "\<And>s x. g (r' x s) = g s" and gp': "\<And>s x. g' (r x s) = g' s"
+  assumes z: "\<And>s x x'. r x (const_env (r' x') s) = r' x' (const_env (r x) s)"
+  assumes gp: "\<And>s x. g (const_env (r' x) s) = g s" and gp': "\<And>s x. g' (const_env (r x) s) = g' s"
   assumes efim: "empty_fail im" and efim': "empty_fail im'"
   shows      "do x \<leftarrow> m; y \<leftarrow> m' im'; n x y od = do y \<leftarrow> m' im'; x \<leftarrow> m; n x y od"
   apply (rule submonad_comm[where f'=f' and r'=r', OF x1 _ x2 _ z])
@@ -470,7 +430,8 @@ qed
 
 lemma submonad_singleton:
   "submonad_fn fetch replace \<top> (\<lambda>s. ({(rv s, s' s)}, False))
-     = (\<lambda>s. ({(rv (fetch s), replace (s' (fetch s)) s)}, False))"
+     = (\<lambda>s. ({(rv (monad_state () (fetch s)),
+              mstate (replace (s' (monad_state () (fetch s))) s))}, False))"
   apply (rule ext)
   apply (simp add: submonad_fn_def bind_def gets_def
                 put_def get_def modify_def return_def
@@ -478,15 +439,15 @@ lemma submonad_singleton:
   done
 
 lemma gets_submonad:
-  "\<lbrakk> submonad_args fetch replace \<top>; \<And>s. f s = f' (fetch s); m = gets f' \<rbrakk>
+  "\<lbrakk> submonad_args fetch replace \<top>; \<And>s. f s = f' (monad_state () (fetch s)); m = gets f' \<rbrakk>
    \<Longrightarrow> gets f = submonad_fn fetch replace \<top> m"
   apply (drule submonad_args.args(3))
   apply (clarsimp simp add: simpler_gets_def submonad_singleton)
   done
 
 lemma modify_submonad:
-  "\<lbrakk> \<And>s. f s = replace (K_record (f' (fetch s))) s; m = modify f' \<rbrakk>
-     \<Longrightarrow> modify f = submonad_fn fetch (replace o K_record) \<top> m"
+  "\<lbrakk> \<And>s. f s = replace (mstate (f' (monad_state () (fetch s)))) s; m = modify f' \<rbrakk>
+     \<Longrightarrow> modify f = submonad_fn fetch replace \<top> m"
   by (simp add: simpler_modify_def submonad_singleton)
 
 lemma fail_submonad:
@@ -515,15 +476,10 @@ lemma is_stateAssert_gets:
   apply (rule ext)
   apply (clarsimp simp: bind_def empty_fail_def valid_def no_fail_def
                         stateAssert_def assert_def gets_def get_def
-                        return_def fail_def image_def split_def)
-  apply (case_tac "f x")
-  apply (intro conjI impI)
-   apply (drule_tac x=x in spec)+
-   apply (subgoal_tac "\<forall>xa\<in>fst (f x). fst xa = fetch x \<and> snd xa = x")
-    apply fastforce
-   apply clarsimp
+                        return_def fail_def)
   apply (drule_tac x=x in spec)+
-  apply fastforce
+  apply (case_tac "f x", clarsimp)
+  apply (intro conjI impI; fastforce) (* faster than fastforce alone *)
   done
 
 lemma is_modify:
@@ -539,8 +495,8 @@ lemma is_modify:
 
 lemma submonad_comm':
   assumes sm1: "submonad f r g m" and sm2: "submonad f' r' g' m'"
-  assumes z: "\<And>s x x'. r x (r' x' s) = r' x' (r x s)"
-  assumes gp: "\<And>s x. g (r' x s) = g s" and gp': "\<And>s x. g' (r x s) = g' s"
+  assumes z: "\<And>s x x'. r x (const_env (r' x') s) = r' x' (const_env (r x) s)"
+  assumes gp: "\<And>s x. g (const_env (r' x) s) = g s" and gp': "\<And>s x. g' (const_env (r x) s) = g' s"
   assumes efim: "empty_fail im" and efim': "empty_fail im'"
   shows      "(do x \<leftarrow> m im; y \<leftarrow> m' im'; n x y od) =
               (do y \<leftarrow> m' im'; x \<leftarrow> m im; n x y od)"
